revised most calls to check_vprop to instead rely on metatheorems and the typing of the post hint

pulse/lib/steel/pulse/Pulse.Checker.Bind.fst
@@ -130,7 +130,7 @@ let check_bind
   (t:st_term{Tm_Bind? t.term})
   (pre:term)
   (pre_typing:tot_typing g pre Tm_VProp)
-  (post_hint:option term)
+  (post_hint:post_hint_opt g)
   (check:check_t)
   : T.Tac (t:st_term &
            c:comp { stateful_comp c ==> comp_pre c == pre } &
@@ -145,40 +145,40 @@ let check_bind
     let t = s1.res in
     let s1_typing = Metatheory.comp_typing_inversion c1_typing in
     let (| t_typing, _, x, next_pre_typing |) = Metatheory.st_comp_typing_inversion s1_typing in
-    (
-        let px = b.binder_ppname, x in
-        let next_pre = open_term_nv s1.post px in
+    let px = b.binder_ppname, x in
+    let next_pre = open_term_nv s1.post px in
         // T.print (Printf.sprintf "Bind::e1 %s \n\nx %s\n\ne2 %s\n\nnext_pre %s\n\n"
         //            (P.term_to_string e1)
         //            (string_of_int x)
         //            (P.term_to_string (open_term e2 x))
         //            (P.term_to_string next_pre));
-        let g' = extend x (Inl s1.res) g in
-        let (| e2', c2, d2 |) = check g' (open_st_term_nv e2 px) next_pre next_pre_typing post_hint in
-        FV.st_typing_freevars d2;
-        if C_Tot? c2
-        then T.fail "Bind: c2 is not st"
-        else
-          let e2_closed = close_st_term e2' x in
-          assume (open_st_term e2_closed x == e2');
-          let d2 : st_typing g' e2' c2 = d2 in
-          let d2 : st_typing g' (open_st_term e2_closed x) c2 = d2 in
-          let s2 = st_comp_of_comp c2 in
-          (* this next check is unavoidable, since we need to type the result in a smaller env g *)          
-          let (| u, res_typing |) = check_universe g s2.res in 
-          if not (eq_univ u s2.u)
-          then T.fail "Unexpected universe for result type"
-          else if x `Set.mem` freevars s2.post
-          then T.fail (Printf.sprintf "Bound variable %d escapes scope in postcondition %s" x (P.term_to_string s2.post))
-          else (
-            let y = x in //fresh g in
-            let s2_post_opened = open_term_nv s2.post (v_as_nv y) in
-            let post_typing = check_vprop_with_core (extend y (Inl s2.res) g) s2_post_opened in
-            //assume (~ (x `Set.mem` freevars_st e2_closed));
-            mk_bind g pre e1 e2_closed c1 c2 px d1 t_typing d2 res_typing post_typing
-          )
+    let g' = extend x (Inl s1.res) g in
+    let (| e2', c2, d2 |) = check g' (open_st_term_nv e2 px) next_pre next_pre_typing post_hint in
+    FV.st_typing_freevars d2;
+    if C_Tot? c2
+    then T.fail "Bind: c2 is not st"
+    else (
+      let e2_closed = close_st_term e2' x in
+      assume (open_st_term e2_closed x == e2');
+      let d2 : st_typing g' e2' c2 = d2 in
+      let d2 : st_typing g' (open_st_term e2_closed x) c2 = d2 in
+      let s2 = st_comp_of_comp c2 in
+      (* this next check is unavoidable, since we need to type the result in a smaller env g *)          
+      let (| u, res_typing |) = check_universe g s2.res in 
+      if not (eq_univ u s2.u)
+      then T.fail "Unexpected universe for result type"
+      else if x `Set.mem` freevars s2.post
+      then T.fail (Printf.sprintf "Bound variable %d escapes scope in postcondition %s" x (P.term_to_string s2.post))
+      else (
+        let y = x in //fresh g in
+        let s2_post_opened = open_term_nv s2.post (v_as_nv y) in
+        let post_typing = check_vprop_with_core (extend y (Inl s2.res) g) s2_post_opened in
+        //assume (~ (x `Set.mem` freevars_st e2_closed));
+        mk_bind g pre e1 e2_closed c1 c2 px d1 t_typing d2 res_typing post_typing
+      )
     )
 #pop-options
+//F* takes a long time to compute a VC for the definition above^. Z3 finishes the proof quickly
 
 let check_tot_bind g t pre pre_typing post_hint check =
   let Tm_TotBind { head=e1; body=e2 } = t.term in
