pulse/lib/steel/pulse/Pulse.Checker.Common.fsti
@@ -8,23 +8,99 @@ open Pulse.Syntax
 open Pulse.Elaborate.Pure
 open Pulse.Typing
 module RU = Pulse.RuntimeUtils
-// val force_st (#f:_) (#g:_) (#t:_) (#pre:term)
-//              (pre_typing:tot_typing f g pre Tm_VProp)
-//              (_:(c:comp { stateful_comp c ==> comp_pre c == pre } & 
-//                  st_typing f g t c))
-//   : T.Tac (c:comp_st { comp_pre c == pre } &
-//            st_typing f g t c)
+module Metatheory = Pulse.Typing.Metatheory
 
 
 let push_context (ctx:string) (g:env) : (g':env { g == g' })
   = {g with ctxt = RU.extend_context ctx g.ctxt}
 
+let mk_abs ty t = RT.(mk_abs (elab_term ty) T.Q_Explicit (elab_term t))
+let mk_arrow ty t = RT.mk_arrow (elab_term ty) T.Q_Explicit (elab_term t)
+
+noeq
+type post_hint_t = {
+  g:env;
+  ret_ty:term;
+  u:universe;
+  ty_typing:universe_of g ret_ty u;
+  post:term;
+  post_typing:RT.tot_typing (elab_env g) (mk_abs ret_ty post) (mk_arrow ret_ty Tm_VProp)
+}
+
+
+let env_extends (g' g:env) = 
+  g'.f == g.f /\
+  (exists suffix. suffix @ g.g == g'.g)
+
+let extends_env_trans (g2 g1 g:env) 
+  : Lemma 
+    (requires g2 `env_extends` g1 /\ 
+              g1 `env_extends` g)
+    (ensures g2 `env_extends` g)
+  = eliminate exists suffix2. suffix2 @ g1.g == g2.g
+    returns _
+    with _. (
+      eliminate exists suffix1. suffix1 @ g.g == g1.g
+      returns exists suffix. suffix @ g.g == g2.g
+      with _. (
+        assert (suffix2@(suffix1@g.g) == g2.g);
+        List.Tot.Properties.append_assoc suffix2 suffix1 g.g
+      )
+    )
+
+let extends_extends_env (g:env) (x:var) (b:binding)
+  : Lemma 
+    (ensures (extend x b g) `env_extends` g)
+  = assert ([x,b]@g.g == (extend x b g).g)
+
+let extends_env_refl (g:env)
+  : Lemma 
+    (ensures g `env_extends` g)
+  = assert ([]@g.g == g.g)
+  
+let env_extends_one_trans (g' g:env) (x:var) (b:binding)
+  : Lemma 
+    (requires g' `env_extends` g)
+    (ensures (extend x b g') `env_extends` g)
+  = extends_extends_env g' x b;
+    extends_env_trans (extend x b g') g' g
+
+let post_hint_for_env_p (g:env) (p:post_hint_t) = g `env_extends` p.g
+
+let post_hint_for_env_extends (g:env) (p:post_hint_t) (x:var) (b:binding)
+  : Lemma
+    (requires post_hint_for_env_p g p)
+    (ensures post_hint_for_env_p (extend x b g) p)
+    [SMTPat (post_hint_for_env_p (extend x b g) p)]
+  = env_extends_one_trans g p.g x b
+  
+let post_hint_for_env (g:env) = p:post_hint_t { post_hint_for_env_p g p }
+let post_hint_opt (g:env) = o:option post_hint_t { None? o \/ post_hint_for_env_p g (Some?.v o) }
+
+noeq
+type post_hint_typing_t (g:env) (p:post_hint_t) (x:var) = {
+  ty_typing:universe_of g p.ret_ty p.u;
+  post_typing:tot_typing (extend x (Inl p.ret_ty) g) (open_term p.post x) Tm_VProp
+}
+
+val post_hint_typing (g:env)
+                     (p:post_hint_for_env g)
+                     (x:var { Metatheory.fresh_wrt x g (freevars p.post) })
+  : post_hint_typing_t g p x
+
+val intro_post_hint (g:env) (ret_ty:option term) (post:term)
+  : T.Tac (post_hint_for_env g)
+
+val post_hint_from_comp_typing (#g:env) (#c:comp_st) (ct:Metatheory.comp_typing_u g c)
+  : post_hint_for_env g
+  
 type check_t =
   g:env ->
   t:st_term ->
   pre:term ->
   pre_typing:tot_typing g pre Tm_VProp ->
-  post_hint:option term ->
+  post_hint:post_hint_opt g ->
   T.Tac (t:st_term &
          c:comp{stateful_comp c ==> comp_pre c == pre} &
          st_typing g t c)
+
