pulse/lib/steel/pulse/Pulse.Typing.Metatheory.fst
@@ -3,19 +3,49 @@ open Pulse.Syntax
 open Pulse.Syntax.Naming
 open Pulse.Typing
 
+let admit_st_comp_typing (g:env) (st:st_comp) 
+  : st_comp_typing g st
+  = admit(); 
+    STC g st (fresh g) (admit()) (admit()) (admit())
+
+let admit_comp_typing (g:env) (c:comp_st)
+  : comp_typing_u g c
+  = match c with
+    | C_ST st ->
+      CT_ST g st (admit_st_comp_typing g st)
+    | C_STAtomic inames st ->
+      CT_STAtomic g inames st (admit()) (admit_st_comp_typing g st)
+    | C_STGhost inames st ->
+      CT_STGhost g inames st (admit()) (admit_st_comp_typing g st)      
+
 let st_typing_correctness (#g:env) (#t:st_term) (#c:comp_st) 
                           (_:st_typing g t c)
   : comp_typing_u g c
-  = admit()
-
+  = admit_comp_typing g c
+    
 let add_frame_well_typed (#g:env) (#c:comp_st) (ct:comp_typing_u g c)
                          (#f:term) (ft:tot_typing g f Tm_VProp)
   : comp_typing_u g (add_frame c f)
-  = admit()
+  = admit_comp_typing _ _
 
-let comp_typing_inversion #g #c ct = admit()
+let comp_typing_inversion #g #c ct = 
+  match ct with
+  | CT_ST _ _ st
+  | CT_STAtomic _ _ _ _ st 
+  | CT_STGhost _ _ _ _ st   -> st
 
-let st_comp_typing_inversion_cofinite (#g:env) (#st:_) (ct:st_comp_typing g st) = admit()
+let st_comp_typing_inversion_cofinite (#g:env) (#st:_) (ct:st_comp_typing g st) = 
+  admit(), admit(), (fun _ -> admit())
 
-let st_comp_typing_inversion (#g:env) (#st:_) (ct:st_comp_typing g st) = admit()
+let st_comp_typing_inversion (#g:env) (#st:_) (ct:st_comp_typing g st) = 
+  let STC g st x ty pre post = ct in
+  (| ty, pre, x, post |)
+
+let tm_exists_inversion (#g:env) (#u:universe) (#ty:term) (#p:term) 
+                        (_:tot_typing g (Tm_ExistsSL u ty p should_elim_false) Tm_VProp)
+                        (x:var { fresh_wrt x g (freevars p) } )
+  : universe_of g ty u &
+    tot_typing (extend x (Inl ty) g) p Tm_VProp
+  = admit(), admit()
+
 
